\newcommand{\deriv}[2]{\frac{\partial #1}{\partial #2}}

\newcommand{\backpropStudSolA}{
\begin{align*}
\sigma(x)&=\frac{1}{1+e^{-x}}\\
\frac{\partial \sigma(x)}{\partial x}&=\frac{\partial }{\partial x}\frac{1}{1+e^{-x}}\\
&=\frac{e^{-x}}{(1+e^{-x})^2}\\
&=\frac{1}{1+e^{-x}}\frac{e^{-x}}{1+e^{-x}}\\
&=\sigma(x)\frac{1+e^{-x}-1}{1+e^{-x}}\\
&=\sigma(x)(\frac{1+e^{-x}}{1+e^{-x}}-\frac{1}{1+e^{-x}})\\
&=\sigma(x)(1-\sigma(x))\\
\end{align*}
}

\newcommand{\backpropStudSolB}{
\begin{align*}
c_k &= g(h_k) \\
\delta_k &= \deriv{E}{h_k} \\
&= \deriv{}{h_k} (\frac{1}{2}\sum_{k}(c_k-t_k)^2) \\
&= \sum_{k}\big((c_k-t_k)g'(h_k)\big) \\
\end{align*}
}

\newcommand{\backpropStudSolC}{
\begin{align*}
h_k &= \sum_{j}(w_{jk}b_{j}) + f_{k} \\
\deriv{E}{w_{jk}} &= \deriv{E}{h_k} \deriv{h_k}{w_{jk}} \\
&=\delta_k \deriv{h_k}{w_{jk}} \\
&=\delta_k \deriv{}{w_{jk}}\big(\sum_{j}(w_{jk}b_{j}) + f_{k}\big) \\
&=\delta_k \sum_{j}b_{j} \\
\end{align*}
}

\newcommand{\backpropStudSolD}{
\begin{align*}
h_k &= \sum_{j}(w_{jk}b_{j}) + f_{k} \\
\deriv{E}{f_{k}} &= \deriv{E}{h_k} \deriv{h_k}{f_{k}} \\
&=\delta_k \deriv{h_k}{f_{k}} \\
&=\delta_k \deriv{}{f_{k}}\big(\sum_{j}(w_{jk}b_{j}) + f_{k}\big) \\
&=\delta_k \\
\end{align*}
}

\newcommand{\backpropStudSolE}{
\begin{align*}
h_k &= \sum_{j}(w_{jk}b_{j}) + f_{k} \\
\deriv{h_k}{b_j} &= \sum_{j}w_{jk} \\
\end{align*}
\begin{align*}
b_j &= g(z_j) \\
\psi_j &= \deriv{E}{z_j} \\
&= \deriv{E}{h_k} \deriv{h_k}{b_j}  \deriv{b_j}{z_j}  \\
&= \delta_k \sum_{j}\big(w_{jk} g'(z_j)\big) \\
\end{align*}
}

\newcommand{\backpropStudSolF}{
\begin{align*}
z_j &= \sum_{i}(u_{ij}a_{i}) + e_j \\
\deriv{E}{u_{ij}} &= \deriv{E}{z_j} \deriv{z_j}{u_{ij}} \\
&=\psi_j \deriv{z_j}{u_{ij}}\\
&=\psi_j \deriv{}{u_{ij}}\big(\sum_{i}(u_{ij}a_{i}) + e_j\big) \\
&=\psi_j \sum_{i}a_{i} \\
\end{align*}
}

\newcommand{\backpropStudSolH}{
\begin{align*}
z_j &= \sum_{i}(u_{ij}a_{i}) + e_j \\
\deriv{E}{e_j} &= \deriv{E}{z_j} \deriv{z_j}{e_j} \\
&=\psi_j \deriv{z_j}{e_j}\\
&=\psi_j \deriv{}{e_j}\big(\sum_{i}(u_{ij}a_{i}) + e_j\big) \\
&=\psi_j \\
\end{align*}
}

